the first few SepTests are working!
- seems to be an issue with unification variables,
  probably dealing with vm_compute and meta variables.

MirrorCharge!/src/CancellerTac.v
@@ -1,3 +1,4 @@
+Require Import ExtLib.Core.RelDec.
 Require Import MirrorCore.SymI.
 Require Import MirrorCore.EnvI.
 Require Import MirrorCore.Ext.Expr.
@@ -202,15 +203,16 @@ Section SepLogBuilder.
   Require Import ILogicFunc.
 
   Variable ts : types.
+  (** TODO: Can I eliminate these? **)
   Variables (FM : fun_map ts) (LM : logic_ops ts) (EM : embed_ops ts).
   Let func := ilfunc.
   Local Instance RSym_func : RSym (typD ts) func := @RSym_ilfunc ts FM LM EM.
 
-  Record ConcreteSepLog tySL (BILO : BILOperators (typD ts nil tySL)) : Type :=
+  Record ConcreteSepLog : Type :=
   { ctor_star : func ; ctor_emp : func }.
 
   Record ConcreteSepLogOk tySL (BILO : BILOperators (typD ts nil tySL))
-         (CSL : @ConcreteSepLog tySL BILO) : Type :=
+         (CSL : ConcreteSepLog) : Type :=
   { starOk : forall us tvs,
     exprD' us tvs (Inj CSL.(ctor_star)) (tyArr tySL (tyArr tySL tySL)) =
     Some (fun _ => sepSP)
@@ -224,8 +226,436 @@ Section SepLogBuilder.
   (** NOTE: My [ILogic] must come form LM **)
   Variable (tySL : typ).
   Variable (OPS : ILogicOps (typD ts nil tySL)).
-  Hypothesis LM_OPS : LM tySL = Some OPS.
+  Hypothesis LM_OPS : LM tySL = Some OPS. (** TODO: Is there a way to eliminate this? **)
   Variable (BILO : BILOperators (typD ts nil tySL)).
+  Variable (csl : ConcreteSepLog).
+  Variable (cslOk : @ConcreteSepLogOk tySL BILO csl).
+
+  Variable PureOp : @Pure.PureOp (typD ts nil tySL).
+  Variable PureLaws : @Pure.Pure _ OPS BILO PureOp.
+
+  Definition SepLogSpec_ConcreteSepLog : SepLogSpec func :=
+  {| is_pure := fun _ => false
+   ; is_emp := func_eq csl.(ctor_emp)
+   ; is_star := func_eq csl.(ctor_star)
+  |}.
+
+  Theorem SepLogSpecOk_ConcreteSepLog
+  : @SepLogSpecOk ts _ RSym_func tySL SepLogSpec_ConcreteSepLog OPS BILO.
+  Proof.
+    refine (@Build_SepLogSpecOk _ _ _ _ _ _ _ PureOp PureLaws _ _ _).
+    abstract (inversion 1).
+    abstract (simpl; intros; unfold func_eq in H;
+              consider (RelDec.rel_dec (equ := @eq ilfunc) (ctor_emp csl) e);
+              intros; subst;
+              unfold exprD; destruct (split_env vs);
+              rewrite (cslOk.(empOk) us x); reflexivity).
+    abstract (simpl; intros; unfold func_eq in H;
+              consider (RelDec.rel_dec (equ := @eq ilfunc) (ctor_star csl) e);
+              intros; subst;
+              unfold exprD; destruct (split_env vs);
+              rewrite (cslOk.(starOk) us x); reflexivity).
+  Defined.
+
+  Definition SynSepLog_ConcreteSepLog : SynSepLog ilfunc :=
+  {| e_star := fun (a b : expr ilfunc) => App (App (Inj csl.(ctor_star)) a) b
+   ; e_emp := Inj csl.(ctor_emp)
+   ; e_true := Inj (ilf_true tySL)
+   ; e_and := fun (a b : expr ilfunc) =>
+                App (App (Inj (ilf_and tySL)) a) b
+   |}.
+
+  Definition SynSepLog_ConcreteSepLog_smart : SynSepLog ilfunc :=
+  {| e_star := fun (a b : expr ilfunc) =>
+                 if a ?[ eq ] (Inj csl.(ctor_emp)) then b
+                 else if b ?[ eq ] (Inj csl.(ctor_emp)) then a
+                      else App (App (Inj csl.(ctor_star)) a) b
+   ; e_emp := Inj csl.(ctor_emp)
+   ; e_true := Inj (ilf_true tySL)
+   ; e_and := fun (a b : expr ilfunc) =>
+                if a ?[ eq ] (Inj (ilf_true tySL)) then b
+                else if b ?[ eq ] (Inj (ilf_true tySL)) then a
+                     else App (App (Inj (ilf_and tySL)) a) b
+   |}.
+
+  Hypothesis LMok : logic_opsOk LM.
+
+  Local Instance ILogic_OPS : @ILogic _ OPS.
+  Proof.
+    specialize (LMok tySL).
+    rewrite LM_OPS in LMok. assumption.
+  Defined.
+
+  Lemma typeof_star : typeof_sym (ctor_star csl) = Some (tyArr tySL (tyArr tySL tySL)).
+  Proof.
+    generalize (cslOk.(starOk) nil nil).
+    red_exprD.
+    generalize dependent (symD (ctor_star csl)).
+    forward. inv_all; subst. reflexivity.
+  Qed.
+
+  Theorem typ_eqb_complete : forall x, typ_eqb x x = true.
+  Proof.
+    clear. induction x; simpl; Cases.rewrite_all_goal; auto.
+    { match goal with
+        | |- ?X = _ => consider X
+      end; auto. }
+    { match goal with
+        | |- ?X = _ => consider X
+      end; auto. }
+  Qed.
+
+  Lemma lem_empOk : forall (us : env (typD ts)) (tvs : list typ),
+   exists val : HList.hlist (typD ts nil) tvs -> typD ts nil tySL,
+     exprD' us tvs (e_emp SynSepLog_ConcreteSepLog) tySL = Some val /\
+     (forall vs : HList.hlist (typD ts nil) tvs, val vs -|- empSP).
+  Proof.
+    simpl; intros.
+    eexists. split. apply (cslOk.(empOk) us tvs).
+    intros. reflexivity.
+  Qed.
+
+  Lemma lem_trueOk : forall (us : env (typD ts)) (tvs : list typ),
+   exists val : HList.hlist (typD ts nil) tvs -> typD ts nil tySL,
+     exprD' us tvs (e_true SynSepLog_ConcreteSepLog) tySL = Some val /\
+     (forall vs : HList.hlist (typD ts nil) tvs, val vs -|- ltrue).
+  Proof.
+    simpl; intros.
+    red_exprD.
+    simpl.
+    rewrite LM_OPS.
+    rewrite typ_cast_typ_refl.
+    eexists; split; eauto. simpl. reflexivity.
+  Qed.
+
+  Lemma lem_starOk : forall (us : env (typD ts)) (tvs : list typ) (x y : expr ilfunc)
+     (valx valy : HList.hlist (typD ts nil) tvs -> typD ts nil tySL),
+   exprD' us tvs x tySL = Some valx ->
+   exprD' us tvs y tySL = Some valy ->
+   exists val : HList.hlist (typD ts nil) tvs -> typD ts nil tySL,
+     exprD' us tvs (e_star SynSepLog_ConcreteSepLog x y) tySL = Some val /\
+     (forall vs : HList.hlist (typD ts nil) tvs,
+      val vs -|- valx vs ** valy vs).
+  Proof.
+    simpl; intros.
+    generalize (cslOk.(starOk) us tvs).
+    red_exprD. intros.
+    forward. inv_all; subst.
+    exists (fun g => sepSP (valx g) (valy g)).
+    split; [ | intros; reflexivity ].
+    generalize typeof_star. simpl. intro.
+    rewrite H3. simpl.
+    rewrite exprD'_type_cast in H.
+    rewrite exprD'_type_cast in H0.
+    forward.
+    repeat match goal with
+             | H : ?X = _ |- context [ ?Y ] =>
+               change Y with X ; rewrite H
+           end.
+    inv_all; subst.
+    rewrite typ_eqb_complete.
+    red_exprD.
+    rewrite H3.
+    red_exprD.
+    rewrite H1.
+    repeat match goal with
+             | H : ?X = _ |- context [ ?Y ] =>
+               change Y with X ; rewrite H
+           end.
+    f_equal.
+    change (let K := (fun x g => (x g) (t3 g) (t1 g)) in
+            K (fun _ : HList.hlist (typD ts nil) tvs => t) =
+            K (fun _ : HList.hlist (typD ts nil) tvs => sepSP)).
+    intro. clearbody K. f_equal. auto.
+  Qed.
+
+  Lemma lem_starOk'
+  : forall (us : env (typD ts)) (tvs : list typ) (x y : expr ilfunc)
+           (val : HList.hlist (typD ts nil) tvs -> typD ts nil tySL),
+      exprD' us tvs (e_star SynSepLog_ConcreteSepLog x y) tySL = Some val ->
+      exists valx valy : HList.hlist (typD ts nil) tvs -> typD ts nil tySL,
+        exprD' us tvs x tySL = Some valx /\
+        exprD' us tvs y tySL = Some valy /\
+        (forall vs : HList.hlist (typD ts nil) tvs,
+           val vs -|- valx vs ** valy vs).
+  Proof.
+    simpl; intros.
+    generalize (cslOk.(starOk) us tvs); intros.
+    red_exprD.
+    forward. inv_all; subst.
+    generalize dependent (symD (ctor_star csl)).
+    rewrite typeof_star.
+    simpl. rewrite typ_cast_typ_refl.
+    intros. inv_all; subst.
+    red_exprD.
+    forward. inv_all; subst.
+    simpl in H8.
+    forward. inv_all; subst.
+    assert (t6 = tySL /\ t1 = tySL).
+    { generalize typeof_star. simpl.
+      intro. rewrite H in *.
+      inv_all. auto. }
+    destruct H; subst.
+    do 2 eexists. split; eauto. split; eauto.
+    rewrite cslOk.(starOk) in H3. inv_all. subst.
+    reflexivity.
+  Qed.
+
+  Lemma lem_andOk
+  : forall (us : env (typD ts)) (tvs : list typ) (x y : expr ilfunc)
+           (valx valy : HList.hlist (typD ts nil) tvs -> typD ts nil tySL),
+      exprD' us tvs x tySL = Some valx ->
+      exprD' us tvs y tySL = Some valy ->
+      exists val : HList.hlist (typD ts nil) tvs -> typD ts nil tySL,
+        exprD' us tvs (e_and SynSepLog_ConcreteSepLog x y) tySL = Some val /\
+        (forall vs : HList.hlist (typD ts nil) tvs,
+           val vs -|- valx vs //\\ valy vs).
+  Proof.
+    simpl; intros.
+    red_exprD.
+    rewrite LM_OPS.
+    rewrite exprD'_type_cast in H.
+    forward. inv_all; subst.
+    simpl.
+    rewrite typ_eqb_complete.
+    red_exprD.
+    rewrite LM_OPS.
+    red_exprD.
+    rewrite LM_OPS.
+    rewrite typ_cast_typ_refl.
+    rewrite H2. rewrite H0. eexists; split; eauto.
+    simpl. reflexivity.
+  Qed.
+
+  Lemma lem_andOk'
+  : forall (us : env (typD ts)) (tvs : list typ) (x y : expr ilfunc)
+           (val : HList.hlist (typD ts nil) tvs -> typD ts nil tySL),
+      exprD' us tvs (e_and SynSepLog_ConcreteSepLog x y) tySL = Some val ->
+      exists valx valy : HList.hlist (typD ts nil) tvs -> typD ts nil tySL,
+        exprD' us tvs x tySL = Some valx /\
+        exprD' us tvs y tySL = Some valy /\
+        (forall vs : HList.hlist (typD ts nil) tvs,
+           val vs -|- valx vs //\\ valy vs).
+  Proof.
+    simpl; intros.
+    red_exprD.
+    rewrite LM_OPS in H.
+    forward. inv_all; subst.
+    red_exprD.
+    rewrite LM_OPS in H1.
+    forward. inv_all; subst.
+    red_exprD.
+    simpl in *; rewrite LM_OPS in H.
+    forward. inv_all. subst t4 t0 t t2 p.
+    do 2 eexists; split; eauto. split; eauto.
+    intros.
+    uip_all. reflexivity.
+  Qed.
+
+  Theorem SynSepLogOk_ConcreteSepLog
+  : @SynSepLogOk ts ilfunc _ tySL OPS BILO SynSepLog_ConcreteSepLog.
+  Proof.
+    constructor;
+    eauto using lem_empOk, lem_trueOk, lem_starOk, lem_starOk', lem_andOk, lem_andOk'.
+  Qed.
+
+  Lemma lem_falseOk : forall (us : env (typD ts)) (tvs : list typ),
+   exists val : HList.hlist (typD ts nil) tvs -> typD ts nil tySL,
+     exprD' us tvs (Inj (ilf_false tySL)) tySL = Some val /\
+     (forall vs : HList.hlist (typD ts nil) tvs, val vs -|- lfalse).
+  Proof.
+    simpl; intros.
+    red_exprD.
+    simpl.
+    rewrite LM_OPS.
+    rewrite typ_cast_typ_refl.
+    eexists; split; eauto. simpl. reflexivity.
+  Qed.
+
+  (** TODO: Move to Charge **)
+  Lemma land_lfalseL T OP `{@ILogic T OP} (P : T) : lfalse //\\ P -|- lfalse.
+  Proof.
+    split.
+    { apply landL1. reflexivity. }
+    { apply lfalseL. }
+  Qed.
+
+  Lemma land_lfalseR T OP `{@ILogic T OP} (P : T) : P //\\ lfalse -|- lfalse.
+  Proof.
+    split.
+    { apply landL2. reflexivity. }
+    { apply lfalseL. }
+  Qed.
+
+  Theorem SynSepLogOk_ConcreteSepLog_smart (BIL : @BILogic _ _ BILO)
+  : @SynSepLogOk ts ilfunc _ tySL OPS BILO SynSepLog_ConcreteSepLog_smart.
+  Proof.
+    constructor;
+    eauto using lem_empOk, lem_trueOk, lem_starOk, lem_starOk', lem_andOk, lem_andOk';
+    simpl; intros.
+    { consider (x ?[ eq ] Inj (ctor_emp csl)); intros; subst.
+      { rewrite H0. eexists; split; eauto.
+        intros.
+        destruct (lem_empOk us tvs).
+        simpl in H1. rewrite H in *. destruct H1; inv_all; subst.
+        rewrite H2. rewrite empSPL. reflexivity. }
+      { consider (y ?[ eq ] Inj (ctor_emp csl)); intros; subst.
+        { rewrite H. eexists; split; eauto.
+          intros.
+          destruct (lem_empOk us tvs).
+          simpl in *. rewrite H0 in *. destruct H2; inv_all; subst.
+          rewrite H3. rewrite empSPR; eauto with typeclass_instances. }
+        { eapply lem_starOk; eauto. } } }
+    { consider (x ?[ eq ] Inj (ctor_emp csl)); intros; subst.
+      { rewrite H0.
+        destruct (lem_empOk us tvs) as [ ? [ ? ? ] ].
+        simpl in *. Cases.rewrite_all_goal.
+        do 2 eexists; split; eauto. split; eauto.
+        intros. rewrite H1. rewrite empSPL. reflexivity. }
+      { consider (y ?[ eq ] Inj (ctor_emp csl)); intros; subst.
+        { rewrite H1.
+          destruct (lem_empOk us tvs) as [ ? [ ? ? ] ].
+          simpl in *. Cases.rewrite_all_goal.
+          do 2 eexists; split; eauto. split; eauto.
+          intros. rewrite H2. rewrite empSPR; eauto with typeclass_instances. }
+        { eapply lem_starOk'; eauto. } } }
+    { repeat match goal with
+               | |- context [ exprD' _ _ match ?X with _ => _ end _ ] =>
+                 consider X; intros
+             end; try eapply lem_andOk; eauto;
+      subst; Cases.rewrite_all_goal; eexists; split; eauto; intros.
+      { generalize (lem_trueOk us tvs); simpl.
+        rewrite H. destruct 1 as [ ? [ ? ? ] ].
+        inv_all; subst.
+        rewrite H2. rewrite ltrue_unitL; eauto with typeclass_instances. }
+      { generalize (lem_trueOk us tvs); simpl.
+        rewrite H0. destruct 1 as [ ? [ ? ? ] ].
+        inv_all; subst.
+        rewrite H3. rewrite ltrue_unitR; eauto with typeclass_instances. } }
+    { destruct (lem_trueOk us tvs) as [ ? [ ? ? ] ].
+      simpl in *.
+      repeat match goal with
+               | _ : context [ exprD' _ _ match ?X with _ => _ end _ ] |- _ =>
+                 consider X; intros
+             end; try solve [ eapply lem_andOk'; eauto ]; simpl;
+      subst; Cases.rewrite_all_goal; do 2 eexists; split; eauto; try (split; eauto).
+      { intros. rewrite H1. rewrite ltrue_unitL; eauto with typeclass_instances. }
+      { intros. rewrite H1. rewrite ltrue_unitR; eauto with typeclass_instances. } }
+  Qed.
+
+End SepLogBuilder.
+
+Definition canceller_post
+           (ts : types)
+           (FM : fun_map ts) (LM : logic_ops ts) (EM : embed_ops ts)
+           (tySL : typ)
+           (ILogicOps_SL : ILogicOps (typD ts nil tySL))
+           us vs lhs rhs : Prop :=
+  let rsym := @RSym_ilfunc ts FM LM EM in
+  match @exprD ts ilfunc rsym us vs lhs tySL with
+    | Some lhs0 =>
+      match @exprD ts ilfunc rsym us vs rhs tySL with
+        | Some rhs0 => lhs0 |-- rhs0
+        | None => True
+      end
+    | None => True
+  end.
+
+Definition canceller_pre
+           (ts : types)
+           (FM : fun_map ts) (LM : logic_ops ts) (EM : embed_ops ts)
+           (tySL : typ)
+           (ILogicOps_SL : ILogicOps (typD ts nil tySL))
+           us vs lhs' rhs' sub : Prop :=
+  let rsym := @RSym_ilfunc ts FM LM EM in
+  match @exprD ts ilfunc rsym us vs lhs' tySL with
+    | Some lhs0 =>
+      match @exprD ts ilfunc rsym us vs rhs' tySL with
+        | Some rhs0 =>
+          @Subst.substD
+            (FMapSubst.SUBST.subst ilfunc) (expr ilfunc) typ (typD ts)
+            (Expr_expr rsym)
+            (FMapSubst.SUBST.Subst_subst _)
+            (FMapSubst.SUBST.SubstOk_subst _) us vs sub
+          /\ (lhs0 |-- rhs0)
+        | None => False
+      end
+    | None =>
+      match exprD us vs rhs' tySL with
+        | Some _ => False
+        | None => True
+      end
+  end.
+
+(** This the the final theorem that should be applied.
+ ** Everything is spelled out precisely to avoid ambiguity in applying it.
+ **)
+Theorem apply_the_canceller
+        (ts : types)
+        (FM : fun_map ts) (LM : logic_ops ts) (EM : embed_ops ts)
+        (LMok : logic_opsOk LM) (EMok : embed_opsOk LM EM)
+        (tySL : typ)
+        (ILogicOps_SL : ILogicOps (typD ts nil tySL))
+        (pf : LM tySL = Some ILogicOps_SL)
+        (BILO : BILOperators (typD ts nil tySL))
+        (BIL : BILogic (typD ts nil tySL))
+        (PureOp : @Pure.PureOp (typD ts nil tySL))
+        (PureLaws : @Pure.Pure _ ILogicOps_SL BILO PureOp)
+        (Hpuretrue : Pure.pure ltrue)
+        (CSL : ConcreteSepLog)
+        (CSLok : @ConcreteSepLogOk ts FM LM EM tySL BILO CSL)
+: forall (us vs : env (typD ts)) (lhs rhs lhs' rhs' : expr ilfunc)
+         (sub : SUBST.subst ilfunc),
+    the_canceller (@RSym_func ts FM LM EM) tySL
+                  (@SynSepLog_ConcreteSepLog_smart tySL CSL)
+                  (@SepLogSpec_ConcreteSepLog CSL)
+                  (typeof_env us) (typeof_env vs) lhs rhs (SUBST.subst_empty ilfunc) =
+    (lhs', rhs', sub) ->
+    @canceller_pre ts FM LM EM tySL ILogicOps_SL us vs lhs' rhs' sub ->
+    @canceller_post ts FM LM EM tySL ILogicOps_SL us vs lhs rhs.
+Proof.
+  intros.
+  eapply the_cancellerOk in H; eauto with typeclass_instances.
+  { eapply SynSepLogOk_ConcreteSepLog_smart; eauto. }
+  { unfold SepLogSpec_ConcreteSepLog.
+    instantiate (1 := @SepLogSpecOk_ConcreteSepLog _ _ _ _ _ _ _ _ _ _ _).
+    eapply Hpuretrue. }
+  Grab Existential Variables.
+  eapply CSLok.
+Qed.
+
+
+(**
+Module SepLogBuilder2.
+  Require Import ILogicFunc.
+
+  Variable ts : types.
+  Let func := ilfunc.
+  Variable RSym_func : RSym (typD ts) func.
+
+  Record ConcreteSepLog : Type :=
+  { ctor_star : func ; ctor_emp : func }.
+
+  Variable (tySL : typ).
+  Variable (OPS : ILogicOps (typD ts nil tySL)).
+  Variable (BILO : BILOperators (typD ts nil tySL)).
+
+  Record ConcreteSepLogOk tySL
+
+         (CSL : ConcreteSepLog) : Type :=
+  { starOk : forall us tvs,
+    exprD' us tvs (Inj CSL.(ctor_star)) (tyArr tySL (tyArr tySL tySL)) =
+    Some (fun _ => sepSP)
+  ; empOk : forall us tvs,
+    exprD' us tvs (Inj CSL.(ctor_emp)) tySL = Some (fun _ => empSP)
+  ; trueOk : forall us tvs,
+    exprD' us tvs (Inj (ilf_true tySL)) = Some (fun _ => ltrue)
+  }.
+
+  Definition func_eq : func -> func -> bool :=
+    RelDec.rel_dec (equ := @eq ilfunc).
+
+  (** NOTE: My [ILogic] must come form LM **)
   Variable (csl : @ConcreteSepLog tySL BILO).
   Variable (cslOk : @ConcreteSepLogOk tySL BILO csl).
 
@@ -375,67 +805,4 @@ Section SepLogBuilder.
       uip_all. reflexivity. }
   Qed.
 End SepLogBuilder.
-
-(** This the the final theorem that should be applied.
- ** Everything is spelled out precisely to avoid ambiguity in applying it.
- **)
-Theorem apply_the_canceller
-        (ts : types)
-        (FM : fun_map ts) (LM : logic_ops ts) (EM : embed_ops ts)
-        (LMok : logic_opsOk LM) (EMok : embed_opsOk LM EM)
-        (tySL : typ)
-        (ILogicOps_SL : ILogicOps (typD ts nil tySL))
-        (pf : LM tySL = Some ILogicOps_SL)
-        (BILO : BILOperators (typD ts nil tySL))
-        (BIL : BILogic (typD ts nil tySL))
-        (PureOp : @Pure.PureOp (typD ts nil tySL))
-        (PureLaws : @Pure.Pure _ ILogicOps_SL BILO PureOp)
-        (Hpuretrue : Pure.pure ltrue)
-        (CSL : @ConcreteSepLog ts tySL BILO)
-        (CSLok : @ConcreteSepLogOk ts FM LM EM tySL BILO CSL)
-: forall (us vs : env (typD ts)) (lhs rhs lhs' rhs' : expr ilfunc)
-         (sub : SUBST.subst ilfunc),
-    the_canceller (@RSym_func ts FM LM EM) tySL
-                  (@SynSepLog_ConcreteSepLog ts tySL _ CSL)
-                  (@SepLogSpec_ConcreteSepLog ts tySL BILO CSL)
-                  (typeof_env us) (typeof_env vs) lhs rhs (SUBST.subst_empty ilfunc) =
-    (lhs', rhs', sub) ->
-    (let rsym := @RSym_ilfunc ts FM LM EM in
-    match @exprD ts ilfunc rsym us vs lhs' tySL with
-      | Some lhs0 =>
-        match @exprD ts ilfunc rsym us vs rhs' tySL with
-          | Some rhs0 =>
-            @Subst.substD
-              (FMapSubst.SUBST.subst ilfunc) (expr ilfunc) typ (typD ts)
-              (Expr_expr rsym)
-              (FMapSubst.SUBST.Subst_subst _)
-              (FMapSubst.SUBST.SubstOk_subst _) us vs sub
-            /\ (lhs0 |-- rhs0)
-          | None => False
-        end
-      | None =>
-        match exprD us vs rhs' tySL with
-          | Some _ => False
-          | None => True
-        end
-    end) ->
-    (let rsym := @RSym_ilfunc ts FM LM EM in
-    match @exprD ts ilfunc rsym us vs lhs tySL with
-      | Some lhs0 =>
-        match @exprD ts ilfunc rsym us vs rhs tySL with
-          | Some rhs0 => lhs0 |-- rhs0
-          | None => True
-        end
-      | None => True
-    end).
-Proof.
-  intros.
-  eapply the_cancellerOk in H; eauto with typeclass_instances.
-  { eapply SynSepLogOk_ConcreteSepLog; eauto. }
-  { unfold SepLogSpec_ConcreteSepLog.
-    instantiate (1 := @SepLogSpecOk_ConcreteSepLog _ _ _ _ _ _ _ _ _ _ _).
-    eapply Hpuretrue. }
-  Grab Existential Variables.
-  eapply CSLok.
-  Show Proof.
-Qed.
+**)
